reformulate proof for task 6 termination a bit

isabelle/2024/HSV_tasks_2024.thy
@@ -384,6 +384,34 @@ fun simp_measure :: "query \<Rightarrow> nat"
   where 
     "simp_measure (q :: query) = List.fold (\<lambda> c t. simp_measure_c c + t) q 0"
 
+
+fun in_clause :: "literal \<Rightarrow> clause  \<Rightarrow> bool"
+  where 
+    "in_clause (l :: literal) (c :: clause) = (l \<in> set c)"
+
+fun in_query :: "literal \<Rightarrow> query  \<Rightarrow> bool"
+  where 
+    "in_query (l :: literal) (q :: query) = (list_ex (\<lambda>c. in_clause l c) q)"
+
+
+
+lemma symbol_in_symbol_clause:
+  fixes x :: symbol
+  fixes b :: bool
+  fixes c :: clause 
+  fixes q :: query
+  shows "x \<in> (symbols_clause ((x, b) # c))"
+  by (simp add: symbols_clause_def)
+
+lemma symbol_in_symbol_query:
+  fixes x :: symbol
+  fixes b :: bool
+  fixes c :: clause 
+  fixes q :: query
+  shows "x \<in> (symbols (((x, b) # c) # q))"
+  using symbols_def symbol_in_symbol_clause by auto
+
+
 text \<open> A simple SAT solver. Given a query, it does a three-way case split. If 
   the query has no clauses then it is trivially satisfiable (with the
    empty valuation). If the first clause in the query is empty, then the
@@ -422,16 +450,50 @@ where
 by pat_completeness auto
 termination
 (*
-Effectively, prove that this measure holds for both cases where valuation of x is both T and F
-in the case where (x, b) is an element that is contained within the query
+Plan is to show that there are two cases, where bv = b and where bv \<noteq> b, in both cases, 
+because x \<in> (symbols query), we know that update_query will reduce the overall size of the query
  *)
 proof (relation "measure simp_measure"; clarify; simp_all del: update_query.simps simp_measure.simps)
-  fix x b c q
-  show "simp_measure (update_query (x ::symbol) True (((x, b) # c) # q)) < simp_measure (((x, b) # c) # q)"
-  proof (cases b)
+  fix x b c q bv
+  show "simp_measure (update_query (x :: symbol) (bv :: bool) (((x, b) # c) # q)) < simp_measure (((x, b) # c) # q)"
+    using symbol_in_symbol_query
+  proof (cases "bv = b")
+    case b_case: True
+    then have thesis_split: "simp_measure (update_query x b (((x, b) # c) # q)) = simp_measure (update_query x b [((x, b) # c)]) + simp_measure (update_query x b q)"
+      by (simp add: member_rec(1) update_clause_def)
+    then have uq_eq_uc: "simp_measure (update_query x b [((x, b) # c)]) = simp_measure (update_clause x bv ((x, b) # c))"
+      by (simp add: b_case)
+    then have uc_lt_c: "simp_measure (update_clause x bv ((x, b) # c)) < simp_measure [((x, b) # c)]"
+      using update_clause_def by (simp add: member_rec(1)) (* have proved breakdown of LHS *)
+    (* TODO: break down RHS, then compare their constituent parts *)
+    then have "simp_measure (((x, b) # c) # q) = simp_measure [((x, b) # c)] + simp_measure q" sorry
+    then have "simp_measure (update_query x bv q) < simp_measure q \<Longrightarrow> x \<in> symbols q"
+      using symbol_in_symbol_query symbol_in_symbol_clause try
+    then have "((update_clause x bv ((x, b) # c)) @ q) = update_query x bv q \<Longrightarrow> x \<notin> (symbols q)"
+      using symbol_in_symbol_query symbol_in_symbol_clause try
+    then have "simp_measure ((update_clause x bv ((x, b) # c)) @ q) < simp_measure (((x, b) # c) # q)"
+
+      using simp_measure.simps simp_measure_c.simps member_def try
+    then have "simp_measure (update_query x bv q) \<le> simp_measure q"
+
+      using simp_measure.simps simp_measure_c.simps member_def try
+    then show ?thesis using update_query.simps
+  next
+    case False
+    then show ?thesis sorry
+  qed
+
+
+(*    then have "((update_clause x bv ((x, b) # c)) @ q) = update_query x bv q \<Longrightarrow> x \<notin> (symbols q)" *)
+(*    then have "simp_measure ((update_clause x bv ((x, b) # c)) @ q) = simp_measure (update_query x bv (((x, b) # c) # q)) \<Longrightarrow> x \<notin> (symbols q)" *)
+(*    then have "simp_measure [c] = simp_measure_c c" by simp*)
+
+(* TODO: remove this is if no longer needed
+  proof (cases "x \<in> (symbols q)")
     case True
-    then have "simp_measure (update_query x True (((x, b) # c) # q)) \<le> (simp_measure (((x, b) # c) # q)) - (length c + 1)"
-      sorry
+    then have "x \<in> (symbols_clause c) \<Longrightarrow> x \<in> (symbols q)" by simp
+    then have "(in_query (x, b) q) \<or> (in_query (x, \<not>b) q)" try
+(*"simp_measure (update_query (x ::symbol) True (((x, b) # c) # q)) < simp_measure (((x, b) # c) # q)"*)
    next
     case False
     then show ?thesis sorry
@@ -440,7 +502,7 @@ next
   fix x b c q
   show "simp_measure (update_query x False (((x, b) # c) # q)) < simp_measure (((x, b) # c) # q)"
     sorry
-qed
+qed*)
 
 (* Need to prove that # of Some's = # of elements in q, worst-case (which is still finite)
 Actually, need to prove that # of remaining elements of q to deal with decreases with loops
